src/dafny/beacon/Helpers.cap.dfy
@@ -1,0 +1,80 @@
+// include some essential dependencies
+include "../utils/Eth2Types.dfy"
+include "../utils/MathHelpers.dfy"
+include "../utils/NativeTypes.dfy"
+include "../utils/SetHelpers.dfy"
+include "../utils/SeqHelpers.dfy"
+include "../utils/Helpers.dfy"
+include "../ssz/Constants.dfy"
+
+include "BeaconChainTypes.dfy"
+include "Helpers.s.dfy"
+include "Helpers.p.dfy"
+include "ActiveValidatorBounds.p.dfy"
+include "attestations/AttestationsTypes.dfy"
+include "validators/Validators.dfy"
+
+
+module BeaconHelpersCapella {
+
+    //  Import some constants, types and beacon chain helpers.
+    import opened Eth2Types
+    import opened MathHelpers
+    import opened NativeTypes
+    import opened SetHelpers
+    import opened SeqHelpers
+    import opened Helpers
+    import opened Constants
+
+    import opened BeaconChainTypes
+    import opened BeaconHelperSpec
+    import opened BeaconHelperProofs
+    import opened ActiveValidatorBounds
+    import opened AttestationsTypes
+    import opened Validators
+
+
+    /**
+     * Check if ``validator`` has an 0x01 prefixed "eth1" withdrawal credential.
+     *
+     * @param  validator                A validator.
+     * @return                          True if the validator has an 0x01 prefixed "eth1"
+     */
+    // Define a method to check if a validator has an 0x01 prefixed "eth1" withdrawal credential
+    predicate method has_eth1_withdrawal_credential(validator: Validator)
+    {
+        // Check if the first byte of withdrawal_credentials is equal to the ETH1_ADDRESS_WITHDRAWAL_PREFIX
+        validator.withdrawal_credentials.bs[0] == ETH1_ADDRESS_WITHDRAWAL_PREFIX
+    }
+
+    /**
+     * Check if ``validator`` is fully withdrawable.
+     *
+     * @param validator                A validator.
+     * @param balance                  A Gwei amount.
+     * @param epoch                    An epoch.
+     * @return                         True if the validator is fully withdrawable.
+     */
+    predicate method is_fully_withdrawable_validator(validator: Validator, balance: Gwei, epoch: Epoch)
+    {   
+        has_eth1_withdrawal_credential(validator) &&
+         validator.withdrawable_epoch <= epoch &&
+          balance > 0
+    }
+
+    /**
+     * Check if ``validator`` is partially withdrawable.
+     *
+     * @param validator                A validator.
+     * @param balance                  A Gwei amount.
+     * @param epoch                    An epoch.
+     *
+     * @return                         True if the validator is partially withdrawable.
+     */
+    predicate method is_partially_withdrawable_validator(validator: Validator, balance: Gwei, epoch: Epoch)
+    {
+        has_eth1_withdrawal_credential(validator) &&
+         validator.effective_balance == MAX_EFFECTIVE_BALANCE &&
+          balance > MAX_EFFECTIVE_BALANCE
+    }
+}
